Meta: Ident{T,P} to take name as argument

coq/ZF/Meta/Check.v
@@ -22,8 +22,8 @@ Inductive CheckT (E:Env) : Ctx -> Term -> Ty -> Prop :=
     CheckT E G (Var n) ty
 | CheckHoleT : forall (G:Ctx) (ty:Ty),
     CheckT E G (HoleT ty) ty
-| CheckIdentT : forall (G:Ctx) (name:string) (args:list Term) (tys:list Ty) (ty:Ty),
-    sigT E (Name.local name) = Some (tys,ty) ->
+| CheckIdentT : forall (G:Ctx) (name:Name) (args:list Term) (tys:list Ty) (ty:Ty),
+    sigT E name = Some (tys,ty)              ->
     CheckTs E G args tys                     ->
     CheckT E G (IdentT name args) ty
 | CheckElem : forall (G:Ctx) (x y:Term),
@@ -105,8 +105,8 @@ with CheckP (E:Env) : Ctx -> Proof -> Term -> Prop :=
 | CheckAxiomP : forall (G:Ctx) (t:Term),
     CheckT E G t TyProp                      ->
     CheckP E G (AxiomP t) t
-| CheckIdentP : forall (G:Ctx) (name:string) (args:list Term) (tys:list Ty) (t:Term),
-    sigP E (Name.local name) = Some (tys,t)  ->
+| CheckIdentP : forall (G:Ctx) (name:Name) (args:list Term) (tys:list Ty) (t:Term),
+    sigP E name = Some (tys,t)               ->
     CheckTs E G args tys                     ->
     CheckP E G (IdentP name args) t
 .
