coq/ZF/Meta/Decl/Class/Equiv.v
@@ -35,7 +35,7 @@ Definition equiv : DeclT :=
 (* forall P, equiv P P.                                                         *)
 Definition Refl : DeclP :=
   let concl :=
-    IdentT "equiv" [Var 0; Var 0]
+    IdentT (Name.local "equiv") [Var 0; Var 0]
   in
     {| paraP  := [TyClass]
     ;  conclP := concl
@@ -46,12 +46,12 @@ Definition Refl : DeclP :=
 Definition EquivCompat : DeclP :=
   let concl :=
     Imp
-      (IdentT "equiv" [Var 3; Var 1])
+      (IdentT (Name.local "equiv") [Var 3; Var 1])
       (Imp
-        (IdentT "equiv" [Var 2; Var 0])
+        (IdentT (Name.local "equiv") [Var 2; Var 0])
         (Imp
-          (IdentT "equiv" [Var 3; Var 2])
-          (IdentT "equiv" [Var 1; Var 0])))
+          (IdentT (Name.local "equiv") [Var 3; Var 2])
+          (IdentT (Name.local "equiv") [Var 1; Var 0])))
   in
     {| paraP  := [TyClass; TyClass; TyClass; TyClass]
     ;  conclP := concl
@@ -62,10 +62,10 @@ Definition EquivCompat : DeclP :=
 Definition EquivCompatL : DeclP :=
   let concl :=
     Imp
-      (IdentT "equiv" [Var 2; Var 0])
+      (IdentT (Name.local "equiv") [Var 2; Var 0])
       (Imp
-        (IdentT "equiv" [Var 2; Var 1])
-        (IdentT "equiv" [Var 0; Var 1]))
+        (IdentT (Name.local "equiv") [Var 2; Var 1])
+        (IdentT (Name.local "equiv") [Var 0; Var 1]))
   in
     {| paraP  := [TyClass; TyClass; TyClass]
     ;  conclP := concl
@@ -76,10 +76,10 @@ Definition EquivCompatL : DeclP :=
 Definition EquivCompatR : DeclP :=
   let concl :=
     Imp
-      (IdentT "equiv" [Var 1; Var 0])
+      (IdentT (Name.local "equiv") [Var 1; Var 0])
       (Imp
-        (IdentT "equiv" [Var 2; Var 1])
-        (IdentT "equiv" [Var 2; Var 0]))
+        (IdentT (Name.local "equiv") [Var 2; Var 1])
+        (IdentT (Name.local "equiv") [Var 2; Var 0]))
   in
     {| paraP  := [TyClass; TyClass; TyClass]
     ;  conclP := concl
@@ -90,8 +90,8 @@ Definition EquivCompatR : DeclP :=
 Definition Sym : DeclP :=
   let concl :=
     Imp
-      (IdentT "equiv" [Var 1; Var 0])
-      (IdentT "equiv" [Var 0; Var 1])
+      (IdentT (Name.local "equiv") [Var 1; Var 0])
+      (IdentT (Name.local "equiv") [Var 0; Var 1])
   in
     {| paraP  := [TyClass; TyClass]
     ;  conclP := concl
@@ -102,10 +102,10 @@ Definition Sym : DeclP :=
 Definition Tran : DeclP :=
   let concl :=
     Imp
-      (IdentT "equiv" [Var 2; Var 1])
+      (IdentT (Name.local "equiv") [Var 2; Var 1])
       (Imp
-        (IdentT "equiv" [Var 1; Var 0])
-        (IdentT "equiv" [Var 2; Var 0]))
+        (IdentT (Name.local "equiv") [Var 1; Var 0])
+        (IdentT (Name.local "equiv") [Var 2; Var 0]))
   in
     {| paraP  := [TyClass; TyClass; TyClass]
     ;  conclP := concl
@@ -116,8 +116,8 @@ Definition Tran : DeclP :=
 Definition NotSym : DeclP :=
   let concl :=
     Imp
-      (Not (IdentT "equiv" [Var 1; Var 0]))
-      (Not (IdentT "equiv" [Var 0; Var 1]))
+      (Not (IdentT (Name.local "equiv") [Var 1; Var 0]))
+      (Not (IdentT (Name.local "equiv") [Var 0; Var 1]))
   in
     {| paraP  := [TyClass; TyClass]
     ;  conclP := concl
@@ -131,8 +131,9 @@ Definition EqualToClass : DeclP :=
         (All
           (Iff
             (Equal (Var 1) (Var 0))
-            (IdentT "equiv"
-              [IdentT "toClass" [Var 1]; IdentT "toClass" [Var 0]])))
+            (IdentT (Name.local "equiv")
+              [IdentT (Name.local "toClass") [Var 1];
+               IdentT (Name.local "toClass") [Var 0]])))
   in
     {| paraP  := []
     ;  conclP := concl
@@ -147,8 +148,9 @@ Definition NotEqualToClass : DeclP :=
           (Iff
             (NotEq (Var 1) (Var 0))
             (Not
-              (IdentT "equiv"
-                [IdentT "toClass" [Var 1]; IdentT "toClass" [Var 0]]))))
+              (IdentT (Name.local "equiv")
+                [IdentT (Name.local "toClass") [Var 1];
+                 IdentT (Name.local "toClass") [Var 0]]))))
   in
     {| paraP  := []
     ;  conclP := concl
@@ -159,12 +161,12 @@ Definition NotEqualToClass : DeclP :=
 Definition NotCompat : DeclP :=
   let concl :=
     Imp
-      (IdentT "equiv" [Var 3; Var 2])
+      (IdentT (Name.local "equiv") [Var 3; Var 2])
       (Imp
-        (IdentT "equiv" [Var 1; Var 0])
+        (IdentT (Name.local "equiv") [Var 1; Var 0])
         (Imp
-          (Not (IdentT "equiv" [Var 3; Var 1]))
-          (Not (IdentT "equiv" [Var 2; Var 0]))))
+          (Not (IdentT (Name.local "equiv") [Var 3; Var 1]))
+          (Not (IdentT (Name.local "equiv") [Var 2; Var 0]))))
   in
     {| paraP  := [TyClass; TyClass; TyClass; TyClass]
     ;  conclP := concl
@@ -175,10 +177,10 @@ Definition NotCompat : DeclP :=
 Definition NotCompatL : DeclP :=
   let concl :=
     Imp
-      (IdentT "equiv" [Var 2; Var 1])
+      (IdentT (Name.local "equiv") [Var 2; Var 1])
       (Imp
-        (Not (IdentT "equiv" [Var 2; Var 0]))
-        (Not (IdentT "equiv" [Var 1; Var 0])))
+        (Not (IdentT (Name.local "equiv") [Var 2; Var 0]))
+        (Not (IdentT (Name.local "equiv") [Var 1; Var 0])))
   in
     {| paraP  := [TyClass; TyClass; TyClass]
     ;  conclP := concl
@@ -189,10 +191,10 @@ Definition NotCompatL : DeclP :=
 Definition NotCompatR : DeclP :=
   let concl :=
     Imp
-      (IdentT "equiv" [Var 2; Var 1])
+      (IdentT (Name.local "equiv") [Var 2; Var 1])
       (Imp
-        (Not (IdentT "equiv" [Var 0; Var 2]))
-        (Not (IdentT "equiv" [Var 0; Var 1])))
+        (Not (IdentT (Name.local "equiv") [Var 0; Var 2]))
+        (Not (IdentT (Name.local "equiv") [Var 0; Var 1])))
   in
     {| paraP  := [TyClass; TyClass; TyClass]
     ;  conclP := concl
