coq/ZF/Meta/Decl/Axiom/Choice.v
@@ -23,13 +23,15 @@ Definition Choice : DeclT :=
       All
         (Ex
           (And
-            (IdentT "FunctionOn" [Var 0; Var 1])
+            (IdentT (Name.local "FunctionOn") [Var 0; Var 1])
             (All
               (Imp
                 (Elem (Var 0) (Var 2))
                 (Imp
-                  (NotEq (Var 0) (IdentT "empty" []))
-                  (Elem (IdentT "eval" [Var 1; Var 0]) (Var 0)))))))
+                  (NotEq (Var 0) (IdentT (Name.local "empty") []))
+                  (Elem
+                    (IdentT (Name.local "eval") [Var 1; Var 0])
+                    (Var 0)))))))
   |}.
 
 Definition imports : Env := Env.unions
